{-# OPTIONS --without-K  --safe #-}

open import Definition.Typed.EqualityRelation
open import Tools.Relation

module Definition.LogicalRelation.Substitution.Introductions.Emptyrec {a ℓ} (M′ : Setoid a ℓ)
                                                                      {{eqrel : EqRelSet M′}} where
open EqRelSet {{...}}
open Setoid M′ using (_≈_) renaming (Carrier to M; refl to ≈-refl)

open import Definition.Untyped M as U hiding (wk ; _∷_)
open import Definition.Untyped.Properties M
open import Definition.Typed M′
import Definition.Typed.Weakening M′ as T
open import Definition.Typed.Properties M′
open import Definition.Typed.RedSteps M′
open import Definition.LogicalRelation M′
open import Definition.LogicalRelation.ShapeView M′
open import Definition.LogicalRelation.Irrelevance M′
open import Definition.LogicalRelation.Properties M′
open import Definition.LogicalRelation.Application M′
open import Definition.LogicalRelation.Substitution M′
open import Definition.LogicalRelation.Substitution.Properties M′
import Definition.LogicalRelation.Substitution.Irrelevance M′ as S
open import Definition.LogicalRelation.Substitution.Reflexivity M′
open import Definition.LogicalRelation.Substitution.Weakening M′
open import Definition.LogicalRelation.Substitution.Introductions.Empty M′
open import Definition.LogicalRelation.Substitution.Introductions.Pi M′
open import Definition.LogicalRelation.Substitution.Introductions.SingleSubst M′

open import Tools.Product
open import Tools.Unit
open import Tools.Empty
open import Tools.Nat

import Tools.PropositionalEquality as PE

private
  variable
    m n : Nat
    Γ : Con Term n
    Δ : Con Term m
    p p′ : M

-- Empty elimination closure reduction (requires reducible terms and equality).
Emptyrec-subst* : ∀ {C n n′ l}
              → Γ ⊢ C
              → Γ ⊢ n ⇒* n′ ∷ Empty
              → ([Empty] : Γ ⊩⟨ l ⟩ Empty)
              → Γ ⊩⟨ l ⟩ n′ ∷ Empty / [Empty]
              → Γ ⊢ Emptyrec p C n ⇒* Emptyrec p C n′ ∷ C
Emptyrec-subst* C (id x) [Empty] [n′] = id (Emptyrecⱼ C x)
Emptyrec-subst* {p = p} C (x ⇨ n⇒n′) [Empty] [n′] =
  let q , w = redSubst*Term n⇒n′ [Empty] [n′]
      a , s = redSubstTerm x [Empty] q
  in  Emptyrec-subst C x ⇨ conv* (Emptyrec-subst* C n⇒n′ [Empty] [n′]) (refl C)

-- Reducibility of empty elimination under a valid substitution.
EmptyrecTerm : ∀ {F n σ l}
             ([Γ]  : ⊩ᵛ Γ)
             ([F]  : Γ ⊩ᵛ⟨ l ⟩ F / [Γ])
             (⊢Δ   : ⊢ Δ)
             ([σ]  : Δ ⊩ˢ σ ∷ Γ / [Γ] / ⊢Δ)
             ([σn] : Δ ⊩⟨ l ⟩ n ∷ Empty / Emptyᵣ (idRed:*: (Emptyⱼ ⊢Δ)))
           → Δ ⊩⟨ l ⟩ Emptyrec p (subst σ F) n
               ∷ subst σ F
               / proj₁ ([F] ⊢Δ [σ])
EmptyrecTerm {Γ = Γ} {Δ = Δ} {F = F} {n} {σ} {l} [Γ] [F] ⊢Δ [σ]
           (Emptyₜ m d n≡n (ne (neNfₜ neM ⊢m m≡m))) =
  let [Empty] = Emptyᵛ {l = l} [Γ]
      [σEmpty] = proj₁ ([Empty] ⊢Δ [σ])
      [σm] = neuTerm [σEmpty] neM ⊢m m≡m
      [σF] = proj₁ ([F] ⊢Δ [σ])
      ⊢F = escape [σF]
      ⊢F≡F = escapeEq [σF] (reflEq [σF])
      EmptyrecM = neuTerm [σF] (Emptyrecₙ neM) (Emptyrecⱼ ⊢F ⊢m)
                        (~-Emptyrec ⊢F≡F m≡m ≈-refl)
      reduction = Emptyrec-subst* ⊢F (redₜ d) [σEmpty] [σm]
  in proj₁ (redSubst*Term reduction [σF] EmptyrecM)


-- Reducibility of empty elimination congruence under a valid substitution equality.
Emptyrec-congTerm : ∀ {F F′ n m σ σ′ l}
                  ([Γ]      : ⊩ᵛ Γ)
                  ([F]      : Γ ⊩ᵛ⟨ l ⟩ F / [Γ])
                  ([F′]     : Γ ⊩ᵛ⟨ l ⟩ F′ / [Γ])
                  ([F≡F′]   : Γ ⊩ᵛ⟨ l ⟩ F ≡ F′ / [Γ] / [F])
                  (⊢Δ       : ⊢ Δ)
                  ([σ]      : Δ ⊩ˢ σ  ∷ Γ / [Γ] / ⊢Δ)
                  ([σ′]     : Δ ⊩ˢ σ′ ∷ Γ / [Γ] / ⊢Δ)
                  ([σ≡σ′]   : Δ ⊩ˢ σ ≡ σ′ ∷ Γ / [Γ] / ⊢Δ / [σ])
                  ([σn]     : Δ ⊩⟨ l ⟩ n ∷ Empty / Emptyᵣ (idRed:*: (Emptyⱼ ⊢Δ)))
                  ([σm]     : Δ ⊩⟨ l ⟩ m ∷ Empty / Emptyᵣ (idRed:*: (Emptyⱼ ⊢Δ)))
                  ([σn≡σm]  : Δ ⊩⟨ l ⟩ n ≡ m ∷ Empty / Emptyᵣ (idRed:*: (Emptyⱼ ⊢Δ)))
                → p ≈ p′
                → Δ ⊩⟨ l ⟩ Emptyrec p (subst σ F) n
                    ≡ Emptyrec p′ (subst σ′ F′) m
                    ∷ subst σ F
                    / proj₁ ([F] ⊢Δ [σ])
Emptyrec-congTerm {Γ = Γ} {Δ = Δ} {p = p} {p′ = p′} {F} {F′} {n} {m} {σ} {σ′} {l}
                [Γ] [F] [F′] [F≡F′]
                ⊢Δ [σ] [σ′] [σ≡σ′]
                (Emptyₜ n′ d n≡n (ne (neNfₜ neN′ ⊢n′ n≡n₁)))
                (Emptyₜ m′ d′ m≡m (ne (neNfₜ neM′ ⊢m′ m≡m₁)))
                (Emptyₜ₌ n″ m″ d₁ d₁′ t≡u (ne (neNfₜ₌ x₂ x₃ prop₂)))
                p≈p′ =
  let n″≡n′ = whrDet*Term (redₜ d₁ , ne x₂) (redₜ d , ne neN′)
      m″≡m′ = whrDet*Term (redₜ d₁′ , ne x₃) (redₜ d′ , ne neM′)
      [Empty] = Emptyᵛ {l = l} [Γ]
      [σEmpty] = proj₁ ([Empty] ⊢Δ [σ])
      [σ′Empty] = proj₁ ([Empty] ⊢Δ [σ′])
      [σF] = proj₁ ([F] ⊢Δ [σ])
      [σ′F] = proj₁ ([F] ⊢Δ [σ′])
      [σ′F′] = proj₁ ([F′] ⊢Δ [σ′])
      [σn′] = neuTerm [σEmpty] neN′ ⊢n′ n≡n₁
      [σ′m′] = neuTerm [σ′Empty] neM′ ⊢m′ m≡m₁
      ⊢F = escape [σF]
      ⊢F≡F = escapeEq [σF] (reflEq [σF])
      ⊢F′ = escape [σ′F′]
      ⊢F′≡F′ = escapeEq [σ′F′] (reflEq [σ′F′])
      ⊢σF≡σ′F = escapeEq [σF] (proj₂ ([F] ⊢Δ [σ]) [σ′] [σ≡σ′])
      ⊢σ′F≡σ′F′ = escapeEq [σ′F] ([F≡F′] ⊢Δ [σ′])
      ⊢F≡F′ = ≅-trans ⊢σF≡σ′F ⊢σ′F≡σ′F′
      [σF≡σ′F] = proj₂ ([F] ⊢Δ [σ]) [σ′] [σ≡σ′]
      [σ′F≡σ′F′] = [F≡F′] ⊢Δ [σ′]
      [σF≡σ′F′] = transEq [σF] [σ′F] [σ′F′] [σF≡σ′F] [σ′F≡σ′F′]
      EmptyrecN = neuTerm [σF] (Emptyrecₙ neN′) (Emptyrecⱼ ⊢F ⊢n′)
                        (~-Emptyrec ⊢F≡F n≡n₁ ≈-refl)
      EmptyrecM = neuTerm [σ′F′] (Emptyrecₙ neM′) (Emptyrecⱼ ⊢F′ ⊢m′)
                        (~-Emptyrec ⊢F′≡F′ m≡m₁ ≈-refl)
      EmptyrecN≡M =
          (neuEqTerm [σF] (Emptyrecₙ neN′) (Emptyrecₙ neM′)
                     (Emptyrecⱼ ⊢F ⊢n′)
                     (conv (Emptyrecⱼ ⊢F′ ⊢m′)
                            (sym (≅-eq (escapeEq [σF]
                              (transEq [σF] [σ′F] [σ′F′] [σF≡σ′F] [σ′F≡σ′F′])))))
                     (~-Emptyrec ⊢F≡F′
                               (PE.subst₂ (λ x y → _ ⊢ x ~ y ∷ _)
                                          n″≡n′ m″≡m′ prop₂)
                               p≈p′))
      reduction₁ = Emptyrec-subst* ⊢F (redₜ d) [σEmpty] [σn′]
      reduction₂ = Emptyrec-subst* ⊢F′ (redₜ d′) [σ′Empty] [σ′m′]
      eq₁ = proj₂ (redSubst*Term reduction₁ [σF] EmptyrecN)
      eq₂ = proj₂ (redSubst*Term reduction₂ [σ′F′] EmptyrecM)
  in  transEqTerm [σF] eq₁
                 (transEqTerm [σF] EmptyrecN≡M
                              (convEqTerm₂ [σF] [σ′F′] [σF≡σ′F′]
                                           (symEqTerm [σ′F′] eq₂)))

-- Validity of empty elimination.
Emptyrecᵛ : ∀ {F n l} ([Γ] : ⊩ᵛ Γ)
          ([Empty]  : Γ ⊩ᵛ⟨ l ⟩ Empty / [Γ])
          ([F]  : Γ ⊩ᵛ⟨ l ⟩ F / [Γ])
        → ([n] : Γ ⊩ᵛ⟨ l ⟩ n ∷ Empty / [Γ] / [Empty])
        → Γ ⊩ᵛ⟨ l ⟩ Emptyrec p F n ∷ F / [Γ] / [F]
Emptyrecᵛ {F = F} {n} {l = l} [Γ] [Empty] [F] [n]
        {Δ = Δ} {σ = σ} ⊢Δ [σ] =
  let [σn] = irrelevanceTerm {l′ = l} (proj₁ ([Empty] ⊢Δ [σ]))
                             (Emptyᵣ (idRed:*: (Emptyⱼ ⊢Δ))) (proj₁ ([n] ⊢Δ [σ]))
  in EmptyrecTerm {F = F} [Γ] [F] ⊢Δ [σ] [σn]
    , λ {σ'} [σ′] [σ≡σ′] →
      let [σ′n] = irrelevanceTerm {l′ = l} (proj₁ ([Empty] ⊢Δ [σ′]))
                                  (Emptyᵣ (idRed:*: (Emptyⱼ ⊢Δ))) (proj₁ ([n] ⊢Δ [σ′]))
          [σn≡σ′n] = irrelevanceEqTerm {l′ = l} (proj₁ ([Empty] ⊢Δ [σ]))
                                       (Emptyᵣ (idRed:*: (Emptyⱼ ⊢Δ)))
                                       (proj₂ ([n] ⊢Δ [σ]) [σ′] [σ≡σ′])
          congTerm = Emptyrec-congTerm {F = F} {F′ = F} [Γ] [F] [F] (reflᵛ {A = F} {l = l} [Γ] [F])
                                       ⊢Δ [σ] [σ′] [σ≡σ′] [σn] [σ′n] [σn≡σ′n] ≈-refl
      in congTerm

-- Validity of empty elimination congruence.
Emptyrec-congᵛ : ∀ {F F′ n n′ l} ([Γ] : ⊩ᵛ Γ)
          ([Empty]  : Γ ⊩ᵛ⟨ l ⟩ Empty / [Γ])
          ([F]  : Γ ⊩ᵛ⟨ l ⟩ F / [Γ])
          ([F′]  : Γ ⊩ᵛ⟨ l ⟩ F′ / [Γ])
          ([F≡F′]  : Γ ⊩ᵛ⟨ l ⟩ F ≡ F′ / [Γ] / [F])
          ([n] : Γ ⊩ᵛ⟨ l ⟩ n ∷ Empty / [Γ] / [Empty])
          ([n′] : Γ ⊩ᵛ⟨ l ⟩ n′ ∷ Empty / [Γ] / [Empty])
          ([n≡n′] : Γ ⊩ᵛ⟨ l ⟩ n ≡ n′ ∷ Empty / [Γ] / [Empty])
        → p ≈ p′
        → Γ ⊩ᵛ⟨ l ⟩ Emptyrec p F n ≡ Emptyrec p′ F′ n′ ∷ F / [Γ] / [F]
Emptyrec-congᵛ {F = F} {F′} {n} {n′} {l = l}
             [Γ] [Empty] [F] [F′] [F≡F′]
             [n] [n′] [n≡n′] p≈p′ {Δ = Δ} {σ = σ} ⊢Δ [σ] =
  let [σn] = irrelevanceTerm {l′ = l} (proj₁ ([Empty] ⊢Δ [σ]))
                             (Emptyᵣ (idRed:*: (Emptyⱼ ⊢Δ))) (proj₁ ([n] ⊢Δ [σ]))
      [σn′] = irrelevanceTerm {l′ = l} (proj₁ ([Empty] ⊢Δ [σ]))
                             (Emptyᵣ (idRed:*: (Emptyⱼ ⊢Δ))) (proj₁ ([n′] ⊢Δ [σ]))
      [σn≡σn′] = irrelevanceEqTerm {l′ = l} (proj₁ ([Empty] ⊢Δ [σ]))
                                   (Emptyᵣ (idRed:*: (Emptyⱼ ⊢Δ))) ([n≡n′] ⊢Δ [σ])
      congTerm = Emptyrec-congTerm {F = F} {F′} [Γ] [F] [F′] [F≡F′]
                                   ⊢Δ [σ] [σ] (reflSubst [Γ] ⊢Δ [σ]) [σn] [σn′] [σn≡σn′] p≈p′
  in congTerm
