{-# OPTIONS --without-K --safe #-}

open import Definition.Typed.EqualityRelation
open import Tools.Relation

module Definition.LogicalRelation.Application {a ℓ} (M′ : Setoid a ℓ)
                                              {{eqrel : EqRelSet M′}} where
open EqRelSet {{...}}
open Setoid M′ using (_≈_) renaming (Carrier to M; refl to ≈-refl)

open import Definition.Untyped M hiding (_∷_)
open import Definition.Untyped.Properties M
open import Definition.Typed M′
open import Definition.Typed.Weakening M′ using (id)
open import Definition.Typed.Properties M′
open import Definition.Typed.RedSteps M′
open import Definition.LogicalRelation M′
open import Definition.LogicalRelation.ShapeView M′
open import Definition.LogicalRelation.Irrelevance M′
open import Definition.LogicalRelation.Properties M′

open import Tools.Nat
open import Tools.Product
import Tools.PropositionalEquality as PE

private
  variable
    n : Nat
    Γ : Con Term n
    p p′ p₁ p₂ q : M

-- Helper function for application of specific type derivations.
appTerm′ : ∀ {F G t u l l′ l″}
          ([F] : Γ ⊩⟨ l″ ⟩ F)
          ([G[u]] : Γ ⊩⟨ l′ ⟩ G [ u ])
          ([ΠFG] : Γ ⊩⟨ l ⟩B⟨ BΠ p q ⟩ Π p , q ▷ F ▹ G)
          ([t] : Γ ⊩⟨ l ⟩ t ∷ Π p , q ▷ F ▹ G / B-intr BΠ! [ΠFG])
          ([u] : Γ ⊩⟨ l″ ⟩ u ∷ F / [F])
        → p ≈ p′
        → Γ ⊩⟨ l′ ⟩ t ∘ p′ ▷ u ∷ G [ u ] / [G[u]]
appTerm′ {Γ = Γ} {p = p} {q = q} {p′ = p′} {t = t} [F] [G[u]] (noemb (Bᵣ F G D ⊢F ⊢G A≡A [F′] [G′] G-ext))
         (Πₜ f d funcF f≡f [f] [f]₁) [u] p≈p′ =
  let ΠFG≡ΠF′G′ = whnfRed* (red D) Πₙ
      F≡F′ , G≡G′ , _ = B-PE-injectivity BΠ! BΠ! ΠFG≡ΠF′G′
      F≡idF′ = PE.trans F≡F′ (PE.sym (wk-id _))
      idG′ᵤ≡Gᵤ = PE.cong (λ x → x [ _ ]) (PE.trans (wk-lift-id _) (PE.sym G≡G′))
      idf∘u≡f∘u = (PE.cong (λ x → x ∘ _ ▷ _) (wk-id _))
      ⊢Γ = wf ⊢F
      [u]′ = irrelevanceTerm′ F≡idF′ [F] ([F′] id ⊢Γ) [u]
      [f∘u] = irrelevanceTerm″ idG′ᵤ≡Gᵤ idf∘u≡f∘u
                                ([G′] id ⊢Γ [u]′) [G[u]] ([f]₁ id ⊢Γ [u]′ p≈p′)
      ⊢u = escapeTerm [F] [u]
      d′ = PE.subst (λ x → Γ ⊢ t ⇒* f ∷ x)
                    (PE.cong₂ (λ F G → Π p′ , q ▷ F ▹ G) (PE.sym F≡F′) (PE.sym G≡G′))
                    (conv* (redₜ d) (Π-cong ⊢F (refl ⊢F) (refl ⊢G) p≈p′ ≈-refl))
  in  proj₁ (redSubst*Term (app-subst* d′ ⊢u) [G[u]] [f∘u])
appTerm′ [F] [G[u]] (emb 0<1 x) [t] [u] = appTerm′ [F] [G[u]] x [t] [u]

-- Application of reducible terms.
appTerm : ∀ {F G t u l l′ l″}
          ([F] : Γ ⊩⟨ l″ ⟩ F)
          ([G[u]] : Γ ⊩⟨ l′ ⟩ G [ u ])
          ([ΠFG] : Γ ⊩⟨ l ⟩ Π p , q ▷ F ▹ G)
          ([t] : Γ ⊩⟨ l ⟩ t ∷ Π p , q ▷ F ▹ G / [ΠFG])
          ([u] : Γ ⊩⟨ l″ ⟩ u ∷ F / [F])
        → p ≈ p′
        → Γ ⊩⟨ l′ ⟩ t ∘ p′ ▷ u ∷ G [ u ] / [G[u]]
appTerm [F] [G[u]] [ΠFG] [t] [u] p≈p′ =
  let [t]′ = irrelevanceTerm [ΠFG] (B-intr BΠ! (Π-elim [ΠFG])) [t]
  in  appTerm′ [F] [G[u]] (Π-elim [ΠFG]) [t]′ [u] p≈p′

-- Helper function for application congruence of specific type derivations.
app-congTerm′ : ∀ {n} {Γ : Con Term n} {F G t t′ u u′ l l′}
          ([F] : Γ ⊩⟨ l′ ⟩ F)
          ([G[u]] : Γ ⊩⟨ l′ ⟩ G [ u ])
          ([ΠFG] : Γ ⊩⟨ l ⟩B⟨ BΠ p q ⟩ Π p , q ▷ F ▹ G)
          ([t≡t′] : Γ ⊩⟨ l ⟩ t ≡ t′ ∷ Π p , q ▷ F ▹ G / B-intr BΠ! [ΠFG])
          ([u] : Γ ⊩⟨ l′ ⟩ u ∷ F / [F])
          ([u′] : Γ ⊩⟨ l′ ⟩ u′ ∷ F / [F])
          ([u≡u′] : Γ ⊩⟨ l′ ⟩ u ≡ u′ ∷ F / [F])
        → p ≈ p₁
        → p ≈ p₂
        → Γ ⊩⟨ l′ ⟩ t ∘ p₁ ▷ u ≡ t′ ∘ p₂ ▷ u′ ∷ G [ u ] / [G[u]]
app-congTerm′ {p = p} {q = q} {p₁ = p₁} {p₂ = p₂} {n = n} {Γ} {F′} {G′} {t = t} {t′ = t′}
              [F] [G[u]] (noemb (Bᵣ F G D ⊢F ⊢G A≡A [F]₁ [G] G-ext))
              (Πₜ₌ f g [ ⊢t , ⊢f , d ] [ ⊢t′ , ⊢g , d′ ] funcF funcG t≡u
                   (Πₜ f′ [ _ , ⊢f′ , d″ ] funcF′ f≡f [f] [f]₁)
                   (Πₜ g′ [ _ , ⊢g′ , d‴ ] funcG′ g≡g [g] [g]₁) [t≡u])
              [a] [a′] [a≡a′] p≈p₁ p≈p₂ =
  let [ΠFG] = Πᵣ′ F G D ⊢F ⊢G A≡A [F]₁ [G] G-ext
      ΠFG≡ΠF′G′ = whnfRed* (red D) Πₙ
      F≡F′ , G≡G′ , _ = B-PE-injectivity BΠ! BΠ! ΠFG≡ΠF′G′
      f≡f′ = whrDet*Term (d , functionWhnf funcF) (d″ , functionWhnf funcF′)
      g≡g′ = whrDet*Term (d′ , functionWhnf funcG) (d‴ , functionWhnf funcG′)
      F≡wkidF′ = PE.trans F≡F′ (PE.sym (wk-id _))
      t∘x≡wkidt∘x : {a b : Term n} {p : M} → wk id a ∘ p ▷ b PE.≡ a ∘ p ▷ b
      t∘x≡wkidt∘x {a} {b} {p} = PE.cong (λ x → x ∘ p ▷ b) (wk-id a)
      t∘x≡wkidt∘x′ : {a : Term n} {p : M} → wk id g′ ∘ p ▷ a PE.≡ g ∘ p ▷ a
      t∘x≡wkidt∘x′ {a} {p} = PE.cong (λ x → x ∘ p ▷ a) (PE.trans (wk-id _) (PE.sym g≡g′))
      wkidG₁[u]≡G[u] = PE.cong (λ x → x [ _ ])
                               (PE.trans (wk-lift-id _) (PE.sym G≡G′))
      wkidG₁[u′]≡G[u′] = PE.cong (λ x → x [ _ ])
                                 (PE.trans (wk-lift-id _) (PE.sym G≡G′))
      ⊢Γ = wf ⊢F
      [u]′ = irrelevanceTerm′ F≡wkidF′ [F] ([F]₁ id ⊢Γ) [a]
      [u′]′ = irrelevanceTerm′ F≡wkidF′ [F] ([F]₁ id ⊢Γ) [a′]
      [u≡u′]′ = irrelevanceEqTerm′ F≡wkidF′ [F] ([F]₁ id ⊢Γ) [a≡a′]
      [G[u′]] = irrelevance′ wkidG₁[u′]≡G[u′] ([G] id ⊢Γ [u′]′)
      [G[u≡u′]] = irrelevanceEq″ wkidG₁[u]≡G[u] wkidG₁[u′]≡G[u′]
                                  ([G] id ⊢Γ [u]′) [G[u]]
                                  (G-ext id ⊢Γ [u]′ [u′]′ [u≡u′]′)
      [f′] : Γ ⊩⟨ _ ⟩ f′ ∷ Π _ , _ ▷ F′ ▹ G′ / [ΠFG]
      [f′] = Πₜ f′ (idRedTerm:*: ⊢f′) funcF′ f≡f [f] [f]₁
      [g′] : Γ ⊩⟨ _ ⟩ g′ ∷ Π _ , _ ▷ F′ ▹ G′ / [ΠFG]
      [g′] = Πₜ g′ (idRedTerm:*: ⊢g′) funcG′ g≡g [g] [g]₁
      [f∘u] = appTerm [F] [G[u]] [ΠFG]
                      (irrelevanceTerm″ PE.refl (PE.sym f≡f′) [ΠFG] [ΠFG] [f′])
                      [a] p≈p₁
      [g∘u′] = appTerm [F] [G[u′]] [ΠFG]
                       (irrelevanceTerm″ PE.refl (PE.sym g≡g′) [ΠFG] [ΠFG] [g′])
                       [a′] p≈p₂
      [tu≡t′u] = irrelevanceEqTerm″ t∘x≡wkidt∘x t∘x≡wkidt∘x wkidG₁[u]≡G[u]
                                     ([G] id ⊢Γ [u]′) [G[u]]
                                     ([t≡u] id ⊢Γ [u]′ p≈p₁ ≈-refl)
      [t′u≡t′u′] = irrelevanceEqTerm″ t∘x≡wkidt∘x′ t∘x≡wkidt∘x′ wkidG₁[u]≡G[u]
                                      ([G] id ⊢Γ [u]′) [G[u]]
                                      ([g] id ⊢Γ [u]′ [u′]′ [u≡u′]′ ≈-refl p≈p₂)
      ΠFG≡ΠF′G′₁ = PE.cong₂ (λ F G → Π p₁ , q ▷ F ▹ G) (PE.sym F≡F′) (PE.sym G≡G′)
      ΠFG≡ΠF′G′₂ = PE.cong₂ (λ F G → Π p₂ , q ▷ F ▹ G) (PE.sym F≡F′) (PE.sym G≡G′)
      d₁ = PE.subst (λ x → Γ ⊢ t ⇒* f ∷ x) ΠFG≡ΠF′G′₁
                    (conv* d (Π-cong ⊢F (refl ⊢F) (refl ⊢G) p≈p₁ ≈-refl))
      d₂ = PE.subst (λ x → Γ ⊢ t′ ⇒* g ∷ x) ΠFG≡ΠF′G′₂
                    (conv* d′ (Π-cong ⊢F (refl ⊢F) (refl ⊢G) p≈p₂ ≈-refl))
      [tu≡fu] = proj₂ (redSubst*Term (app-subst* d₁ (escapeTerm [F] [a]))
                                     [G[u]] [f∘u])
      [gu′≡t′u′] = convEqTerm₂ [G[u]] [G[u′]] [G[u≡u′]]
                     (symEqTerm [G[u′]]
                       (proj₂ (redSubst*Term (app-subst* d₂ (escapeTerm [F] [a′]))
                                             [G[u′]] [g∘u′])))
  in  transEqTerm [G[u]] (transEqTerm [G[u]] [tu≡fu] [tu≡t′u])
                  (transEqTerm [G[u]] [t′u≡t′u′] [gu′≡t′u′])

app-congTerm′ [F] [G[u]] (emb 0<1 x) [t≡t′] [u] [u′] [u≡u′] =
  app-congTerm′ [F] [G[u]] x [t≡t′] [u] [u′] [u≡u′]

-- Application congruence of reducible terms.
app-congTerm : ∀ {F G t t′ u u′ l l′}
          ([F] : Γ ⊩⟨ l′ ⟩ F)
          ([G[u]] : Γ ⊩⟨ l′ ⟩ G [ u ])
          ([ΠFG] : Γ ⊩⟨ l ⟩ Π p , q ▷ F ▹ G)
          ([t≡t′] : Γ ⊩⟨ l ⟩ t ≡ t′ ∷ Π _ , _ ▷ F ▹ G / [ΠFG])
          ([u] : Γ ⊩⟨ l′ ⟩ u ∷ F / [F])
          ([u′] : Γ ⊩⟨ l′ ⟩ u′ ∷ F / [F])
          ([u≡u′] : Γ ⊩⟨ l′ ⟩ u ≡ u′ ∷ F / [F])
        → p ≈ p₁
        → p ≈ p₂
        → Γ ⊩⟨ l′ ⟩ t ∘ p₁ ▷ u ≡ t′ ∘ p₂ ▷ u′ ∷ G [ u ] / [G[u]]
app-congTerm [F] [G[u]] [ΠFG] [t≡t′] p≈p₁ p≈p₂ =
  let [t≡t′]′ = irrelevanceEqTerm [ΠFG] (B-intr BΠ! (Π-elim [ΠFG])) [t≡t′]
  in  app-congTerm′ [F] [G[u]] (Π-elim [ΠFG]) [t≡t′]′ p≈p₁ p≈p₂
