------------------------------------------------------------------------
-- The fundamental lemma of the logical relation for validity.
------------------------------------------------------------------------

open import Definition.Typed.EqualityRelation
open import Definition.Typed.Restrictions
open import Graded.Modality

module Definition.LogicalRelation.Fundamental
  {a} {M : Set a}
  {ğ•„ : Modality M}
  (R : Type-restrictions ğ•„)
  {{eqrel : EqRelSet R}}
  where

open EqRelSet {{...}}
open Type-restrictions R

open import Definition.Untyped M
open import Definition.Untyped.Properties M

open import Definition.Typed R
open import Definition.LogicalRelation R
open import Definition.LogicalRelation.Hidden R
open import Definition.LogicalRelation.Irrelevance R
open import Definition.LogicalRelation.Properties R
open import Definition.LogicalRelation.Substitution R
open import Definition.LogicalRelation.Substitution.Escape R
open import Definition.LogicalRelation.Substitution.Properties R
open import Definition.LogicalRelation.Substitution.Introductions R
import Definition.LogicalRelation.Substitution.Introductions.Erased R
  as Erased
import Definition.LogicalRelation.Substitution.Irrelevance R as S
open import Definition.LogicalRelation.Substitution.Weakening R

import Graded.Derived.Erased.Untyped ğ•„ as E

open import Tools.Function
open import Tools.Level
open import Tools.Product
open import Tools.Unit
open import Tools.Nat using (Nat)
import Tools.PropositionalEquality as PE

private
  variable
    m n : Nat
    Î“ : Con Term n
    Î” : Con Term m
    Ïƒ Ïƒâ‚ Ïƒâ‚‚ Ïƒâ€² : Subst m n
    A Aâ‚ Aâ‚‚ B t tâ‚ tâ‚‚ u : Term _
    âŠ©Î“ : âŠ©áµ› _

opaque
 unfolding _âŠ©áµ›âŸ¨_âŸ©_ _âŠ©áµ›âŸ¨_âŸ©_â‰¡_ _âŠ©áµ›âŸ¨_âŸ©_âˆ·_ _âŠ©áµ›âŸ¨_âŸ©_â‰¡_âˆ·_

 mutual
  -- Fundamental theorem for contexts.
  valid : âŠ¢ Î“ â†’ âŠ©áµ› Î“
  valid Îµ = Îµ
  valid (âŠ¢Î“ âˆ™ A) = let [Î“] , [A] = fundamental A in [Î“] âˆ™ [A]


  -- Fundamental theorem for types.
  fundamental : âˆ€ {A} (âŠ¢A : Î“ âŠ¢ A) â†’ Î£ (âŠ©áµ› Î“) (Î» [Î“] â†’ Î“ âŠ©áµ›âŸ¨ Â¹ âŸ© A / [Î“])
  fundamental (â„•â±¼ âŠ¢Î“) =
    â„•áµ› (valid âŠ¢Î“)
  fundamental (Emptyâ±¼ x) = Emptyáµ› (valid x)
  fundamental (Unitâ±¼ âŠ¢Î“ ok) =
    Unitáµ› (valid âŠ¢Î“) ok
  fundamental (Uâ±¼ âŠ¢Î“) =
    âŠ©áµ›U (valid âŠ¢Î“)
  fundamental (Î Î£â±¼ âŠ¢A âŠ¢B ok) =
    Î Î£áµ› ok (fundamental âŠ¢A) (fundamental âŠ¢B)
  fundamental (Idâ±¼ âŠ¢t âŠ¢u) =
    Idáµ› (fundamentalTerm âŠ¢t) (fundamentalTerm âŠ¢u)
  fundamental (univ âŠ¢A) =
    âŠ©áµ›âˆ·Uâ†’âŠ©áµ› (fundamentalTerm âŠ¢A)

  -- Fundamental theorem for type equality.
  fundamentalEq : âˆ€ {A B} â†’ Î“ âŠ¢ A â‰¡ B
    â†’ âˆƒ  Î» ([Î“] : âŠ©áµ› Î“)
    â†’ âˆƒâ‚‚ Î» ([A] : Î“ âŠ©áµ›âŸ¨ Â¹ âŸ© A / [Î“]) ([B] : Î“ âŠ©áµ›âŸ¨ Â¹ âŸ© B / [Î“])
    â†’ Î“ âŠ©áµ›âŸ¨ Â¹ âŸ© A â‰¡ B / [Î“] / [A]
  fundamentalEq (univ Aâ‰¡B) =
    âŠ©áµ›â‰¡âˆ·Uâ†’âŠ©áµ›â‰¡ (fundamentalTermEq Aâ‰¡B)
  fundamentalEq (refl âŠ¢A) =
    refl-âŠ©áµ›â‰¡ (fundamental âŠ¢A)
  fundamentalEq (sym Aâ‰¡B) =
    sym-âŠ©áµ›â‰¡ (fundamentalEq Aâ‰¡B)
  fundamentalEq (trans Aâ‰¡B Bâ‰¡C) =
    trans-âŠ©áµ›â‰¡ (fundamentalEq Aâ‰¡B) (fundamentalEq Bâ‰¡C)
  fundamentalEq (Î Î£-cong _ Aâ‚â‰¡Aâ‚‚ Bâ‚â‰¡Bâ‚‚ ok) =
    Î Î£-congáµ› ok (fundamentalEq Aâ‚â‰¡Aâ‚‚) (fundamentalEq Bâ‚â‰¡Bâ‚‚)
  fundamentalEq (Id-cong Aâ‚â‰¡Aâ‚‚ tâ‚â‰¡tâ‚‚ uâ‚â‰¡uâ‚‚) =
    Id-congáµ› (fundamentalEq Aâ‚â‰¡Aâ‚‚) (fundamentalTermEq tâ‚â‰¡tâ‚‚)
      (fundamentalTermEq uâ‚â‰¡uâ‚‚)

  -- Fundamental theorem for terms.
  fundamentalTerm : âˆ€ {A t} â†’ Î“ âŠ¢ t âˆ· A
    â†’ âˆƒ Î» ([Î“] : âŠ©áµ› Î“)
    â†’ âˆƒ Î» ([A] : Î“ âŠ©áµ›âŸ¨ Â¹ âŸ© A / [Î“])
    â†’ Î“ âŠ©áµ›âŸ¨ Â¹ âŸ© t âˆ· A / [Î“] / [A]
  fundamentalTerm (â„•â±¼ âŠ¢Î“) =
    â„•áµ—áµ› (valid âŠ¢Î“)
  fundamentalTerm (Emptyâ±¼ x) =
    Emptyáµ—áµ› (valid x)
  fundamentalTerm (Unitâ±¼ âŠ¢Î“ ok) =
    Unitáµ—áµ› (valid âŠ¢Î“) ok
  fundamentalTerm (Î Î£â±¼ {G = B} âŠ¢A âŠ¢B ok) =
    Î Î£áµ—áµ› {B = B} ok (fundamentalTerm âŠ¢A) (fundamentalTerm âŠ¢B)
  fundamentalTerm (var âŠ¢Î“ xâˆˆÎ“) =
    emb-âŠ©áµ›âˆ· â‰¤Â¹ (varáµ› xâˆˆÎ“ (valid âŠ¢Î“) .projâ‚‚)
  fundamentalTerm (lamâ±¼ {t} âŠ¢A âŠ¢t ok) =
    lamáµ› {t = t} ok (fundamental âŠ¢A) (fundamentalTerm âŠ¢t)
  fundamentalTerm (_âˆ˜â±¼_ {t = t} âŠ¢t âŠ¢u) =
    âˆ˜áµ› {t = t} (fundamentalTerm âŠ¢t) (fundamentalTerm âŠ¢u)
  fundamentalTerm (prodâ±¼ {u} _ âŠ¢B âŠ¢t âŠ¢u ok) =
    prodáµ› {u = u} ok (fundamental âŠ¢B) (fundamentalTerm âŠ¢t)
      (fundamentalTerm âŠ¢u)
  fundamentalTerm (fstâ±¼ {t} _ _ âŠ¢t) =
    fstáµ› {t = t} (fundamentalTerm âŠ¢t)
  fundamentalTerm (sndâ±¼ _ _ âŠ¢t) =
    sndáµ› (fundamentalTerm âŠ¢t)
  fundamentalTerm (zeroâ±¼ âŠ¢Î“) =
    zeroáµ› (valid âŠ¢Î“)
  fundamentalTerm (sucâ±¼ {n = t} âŠ¢t) =
    sucáµ› {t = t} (fundamentalTerm âŠ¢t)
  fundamentalTerm (natrecâ±¼ {z = t} {s = u} âŠ¢A âŠ¢t âŠ¢u âŠ¢v) =
    natrecáµ› {t = t} {u = u} (fundamental âŠ¢A) (fundamentalTerm âŠ¢t)
      (fundamentalTerm âŠ¢u) (fundamentalTerm âŠ¢v)
  fundamentalTerm (emptyrecâ±¼ {t = t} âŠ¢A âŠ¢t) =
    emptyrecáµ› {t = t} (fundamental âŠ¢A) (fundamentalTerm âŠ¢t)
  fundamentalTerm (starâ±¼ âŠ¢Î“ ok) =
    staráµ› (valid âŠ¢Î“) ok
  fundamentalTerm (conv {t} âŠ¢t Aâ‰¡B) =
    conv-âŠ©áµ›âˆ· {t = t} (fundamentalEq Aâ‰¡B) (fundamentalTerm âŠ¢t)
  fundamentalTerm (prodrecâ±¼ {u} _ _ âŠ¢C âŠ¢t âŠ¢u _) =
    prodrecáµ› {u = u} (fundamental âŠ¢C) (fundamentalTerm âŠ¢t)
      (fundamentalTerm âŠ¢u)
  fundamentalTerm (unitrecâ±¼ {u} âŠ¢A âŠ¢t âŠ¢u _) =
    unitrecáµ› {u = u} (fundamental âŠ¢A) (fundamentalTerm âŠ¢t)
      (fundamentalTerm âŠ¢u)
  fundamentalTerm (Idâ±¼ {t} {u} âŠ¢A âŠ¢t âŠ¢u) =
    Idáµ—áµ› {t = t} {u = u} (fundamentalTerm âŠ¢A) (fundamentalTerm âŠ¢t)
      (fundamentalTerm âŠ¢u)
  fundamentalTerm (rflâ±¼ âŠ¢t) =
    rfláµ› (fundamentalTerm âŠ¢t)
  fundamentalTerm (Jâ±¼ {u} _ _ âŠ¢B âŠ¢u _ âŠ¢w) =
    Jáµ› {u = u} (fundamental âŠ¢B) (fundamentalTerm âŠ¢u)
      (fundamentalTerm âŠ¢w)
  fundamentalTerm (Kâ±¼ {u} _ âŠ¢B âŠ¢u âŠ¢v ok) =
    Káµ› {u = u} ok (fundamental âŠ¢B) (fundamentalTerm âŠ¢u)
      (fundamentalTerm âŠ¢v)
  fundamentalTerm ([]-congâ±¼ {v} âŠ¢t âŠ¢u âŠ¢v ok) =
    []-congáµ› {v = v} ok (fundamentalTerm âŠ¢v)

  -- Fundamental theorem for term equality.
  fundamentalTermEq : âˆ€ {A t tâ€²} â†’ Î“ âŠ¢ t â‰¡ tâ€² âˆ· A
                    â†’ âˆƒ Î» ([Î“] : âŠ©áµ› Î“) â†’
                      [ Î“ âŠ©áµ›âŸ¨ Â¹ âŸ© t â‰¡ tâ€² âˆ· A / [Î“] ]
  fundamentalTermEq (refl âŠ¢t) =
    refl-âŠ©áµ›â‰¡âˆ· (fundamentalTerm âŠ¢t)
  fundamentalTermEq (sym tâ‰¡u) =
    sym-âŠ©áµ›â‰¡âˆ· (fundamentalTermEq tâ‰¡u)
  fundamentalTermEq (trans tâ‰¡u uâ‰¡v) =
    trans-âŠ©áµ›â‰¡âˆ· (fundamentalTermEq tâ‰¡u) (fundamentalTermEq uâ‰¡v)
  fundamentalTermEq (conv tâ‰¡u Aâ‰¡B) =
    conv-âŠ©áµ›â‰¡âˆ· (fundamentalEq Aâ‰¡B) (fundamentalTermEq tâ‰¡u)
  fundamentalTermEq (Î Î£-cong _ Aâ‚â‰¡Aâ‚‚ Bâ‚â‰¡Bâ‚‚ ok) =
    Î Î£-congáµ—áµ› ok (fundamentalTermEq Aâ‚â‰¡Aâ‚‚) (fundamentalTermEq Bâ‚â‰¡Bâ‚‚)
  fundamentalTermEq (app-cong tâ‚â‰¡tâ‚‚ uâ‚â‰¡uâ‚‚) =
    âˆ˜-congáµ› (fundamentalTermEq tâ‚â‰¡tâ‚‚) (fundamentalTermEq uâ‚â‰¡uâ‚‚)
  fundamentalTermEq (Î²-red _ _ âŠ¢t âŠ¢u PE.refl ok) =
    Î²-redáµ› ok (fundamentalTerm âŠ¢t) (fundamentalTerm âŠ¢u)
  fundamentalTermEq (Î·-eq _ âŠ¢tâ‚ âŠ¢tâ‚‚ wk1-tâ‚âˆ˜0â‰¡wk1-tâ‚‚âˆ˜0) =
    Î·-eqáµ› (fundamentalTerm âŠ¢tâ‚) (fundamentalTerm âŠ¢tâ‚‚)
      (fundamentalTermEq wk1-tâ‚âˆ˜0â‰¡wk1-tâ‚‚âˆ˜0)
  fundamentalTermEq (suc-cong tâ‰¡u) =
    suc-congáµ› (fundamentalTermEq tâ‰¡u)
  fundamentalTermEq (natrec-cong _ Aâ‚â‰¡Aâ‚‚ tâ‚â‰¡tâ‚‚ uâ‚â‰¡uâ‚‚ vâ‚â‰¡vâ‚‚) =
    natrec-congáµ› (fundamentalEq Aâ‚â‰¡Aâ‚‚) (fundamentalTermEq tâ‚â‰¡tâ‚‚)
      (fundamentalTermEq uâ‚â‰¡uâ‚‚) (fundamentalTermEq vâ‚â‰¡vâ‚‚)
  fundamentalTermEq (natrec-zero âŠ¢A âŠ¢t âŠ¢u) =
    natrec-zeroáµ› (fundamental âŠ¢A) (fundamentalTerm âŠ¢t)
      (fundamentalTerm âŠ¢u)
  fundamentalTermEq (natrec-suc âŠ¢A âŠ¢t âŠ¢u âŠ¢v) =
    natrec-sucáµ› (fundamental âŠ¢A) (fundamentalTerm âŠ¢t)
      (fundamentalTerm âŠ¢u) (fundamentalTerm âŠ¢v)
  fundamentalTermEq (emptyrec-cong Fâ‰¡Fâ€² nâ‰¡nâ€²) =
    emptyrec-congáµ› (fundamentalEq Fâ‰¡Fâ€²) (fundamentalTermEq nâ‰¡nâ€²)
  fundamentalTermEq (Î·-unit âŠ¢t âŠ¢u Î·) =
    Î·-unitáµ› (fundamentalTerm âŠ¢t) (fundamentalTerm âŠ¢u) Î·
  fundamentalTermEq (fst-cong _ _ tâ‚â‰¡tâ‚‚) =
    fst-congáµ› (fundamentalTermEq tâ‚â‰¡tâ‚‚)
  fundamentalTermEq (snd-cong _ _ tâ‚â‰¡tâ‚‚) =
    snd-congáµ› (fundamentalTermEq tâ‚â‰¡tâ‚‚)
  fundamentalTermEq (prod-cong _ âŠ¢B tâ‚â‰¡tâ‚‚ uâ‚â‰¡uâ‚‚ ok) =
    prod-congáµ› ok (fundamental âŠ¢B) (fundamentalTermEq tâ‚â‰¡tâ‚‚)
      (fundamentalTermEq uâ‚â‰¡uâ‚‚)
  fundamentalTermEq (Î£-Î²â‚ _ âŠ¢B âŠ¢t âŠ¢u PE.refl ok) =
    Î£-Î²â‚áµ› ok (fundamental âŠ¢B) (fundamentalTerm âŠ¢t) (fundamentalTerm âŠ¢u)
  fundamentalTermEq (Î£-Î²â‚‚ _ âŠ¢B âŠ¢t âŠ¢u PE.refl ok) =
    Î£-Î²â‚‚áµ› ok (fundamental âŠ¢B) (fundamentalTerm âŠ¢t) (fundamentalTerm âŠ¢u)
  fundamentalTermEq (Î£-Î· _ _ âŠ¢tâ‚ âŠ¢tâ‚‚ fst-tâ‚â‰¡fst-tâ‚‚ snd-tâ‚â‰¡snd-tâ‚‚) =
    Î£-Î·áµ› (fundamentalTerm âŠ¢tâ‚) (fundamentalTerm âŠ¢tâ‚‚)
      (fundamentalTermEq fst-tâ‚â‰¡fst-tâ‚‚)
      (fundamentalTermEq snd-tâ‚â‰¡snd-tâ‚‚)
  fundamentalTermEq (prodrec-cong _ _ Câ‚â‰¡Câ‚‚ tâ‚â‰¡tâ‚‚ uâ‚â‰¡uâ‚‚ _) =
    prodrec-congáµ› (fundamentalEq Câ‚â‰¡Câ‚‚) (fundamentalTermEq tâ‚â‰¡tâ‚‚)
      (fundamentalTermEq uâ‚â‰¡uâ‚‚)
  fundamentalTermEq (prodrec-Î² _ _ âŠ¢C âŠ¢t âŠ¢u âŠ¢v PE.refl _) =
    prodrec-Î²áµ› (fundamental âŠ¢C) (fundamentalTerm âŠ¢t)
      (fundamentalTerm âŠ¢u) (fundamentalTerm âŠ¢v)
  fundamentalTermEq (unitrec-cong Aâ‚â‰¡Aâ‚‚ tâ‚â‰¡tâ‚‚ uâ‚â‰¡uâ‚‚ _ _) =
    unitrec-congáµ› (fundamentalEq Aâ‚â‰¡Aâ‚‚) (fundamentalTermEq tâ‚â‰¡tâ‚‚)
      (fundamentalTermEq uâ‚â‰¡uâ‚‚)
  fundamentalTermEq (unitrec-Î² âŠ¢A âŠ¢u _ no-Î·) =
    unitrec-Î²áµ› (fundamental âŠ¢A) (fundamentalTerm âŠ¢u) no-Î·
  fundamentalTermEq (unitrec-Î²-Î· âŠ¢A âŠ¢t âŠ¢u _ Î·) =
    unitrec-Î²-Î·áµ› (fundamental âŠ¢A) (fundamentalTerm âŠ¢t)
      (fundamentalTerm âŠ¢u) Î·
  fundamentalTermEq (Id-cong Aâ‚â‰¡Aâ‚‚ tâ‚â‰¡tâ‚‚ uâ‚â‰¡uâ‚‚) =
    Id-congáµ—áµ› (fundamentalTermEq Aâ‚â‰¡Aâ‚‚) (fundamentalTermEq tâ‚â‰¡tâ‚‚)
      (fundamentalTermEq uâ‚â‰¡uâ‚‚)
  fundamentalTermEq (J-cong _ Aâ‚â‰¡Aâ‚‚ _ tâ‚â‰¡tâ‚‚ Bâ‚â‰¡Bâ‚‚ uâ‚â‰¡uâ‚‚ vâ‚â‰¡vâ‚‚ wâ‚â‰¡wâ‚‚) =
    J-congáµ› (fundamentalEq Aâ‚â‰¡Aâ‚‚) (fundamentalTermEq tâ‚â‰¡tâ‚‚)
      (fundamentalEq Bâ‚â‰¡Bâ‚‚) (fundamentalTermEq uâ‚â‰¡uâ‚‚)
      (fundamentalTermEq vâ‚â‰¡vâ‚‚) (fundamentalTermEq wâ‚â‰¡wâ‚‚)
  fundamentalTermEq (K-cong Aâ‚â‰¡Aâ‚‚ _ tâ‚â‰¡tâ‚‚ Bâ‚â‰¡Bâ‚‚ uâ‚â‰¡uâ‚‚ vâ‚â‰¡vâ‚‚ ok) =
    K-congáµ› ok (fundamentalEq Aâ‚â‰¡Aâ‚‚) (fundamentalTermEq tâ‚â‰¡tâ‚‚)
      (fundamentalEq Bâ‚â‰¡Bâ‚‚) (fundamentalTermEq uâ‚â‰¡uâ‚‚)
      (fundamentalTermEq vâ‚â‰¡vâ‚‚)
  fundamentalTermEq ([]-cong-cong Aâ‚â‰¡Aâ‚‚ tâ‚â‰¡tâ‚‚ uâ‚â‰¡uâ‚‚ vâ‚â‰¡vâ‚‚ ok) =
    []-cong-congáµ› ok (fundamentalEq Aâ‚â‰¡Aâ‚‚) (fundamentalTermEq tâ‚â‰¡tâ‚‚)
      (fundamentalTermEq uâ‚â‰¡uâ‚‚) (fundamentalTermEq vâ‚â‰¡vâ‚‚)
  fundamentalTermEq (J-Î² _ âŠ¢t âŠ¢B âŠ¢u PE.refl) =
    J-Î²áµ› (fundamentalTerm âŠ¢t) (fundamental âŠ¢B) (fundamentalTerm âŠ¢u)
  fundamentalTermEq (K-Î² _ âŠ¢B âŠ¢u ok) =
    K-Î²áµ› ok (fundamental âŠ¢B) (fundamentalTerm âŠ¢u)
  fundamentalTermEq ([]-cong-Î² âŠ¢t PE.refl ok) =
    []-cong-Î²áµ› ok (fundamentalTerm âŠ¢t)

-- Fundamental theorem for substitutions.
fundamentalSubst : (âŠ¢Î“ : âŠ¢ Î“) (âŠ¢Î” : âŠ¢ Î”)
      â†’ Î” âŠ¢Ë¢ Ïƒ âˆ· Î“
      â†’ âˆƒ Î» [Î“] â†’ Î” âŠ©Ë¢ Ïƒ âˆ· Î“ / [Î“] / âŠ¢Î”
fundamentalSubst Îµ âŠ¢Î” [Ïƒ] = Îµ , lift tt
fundamentalSubst (âŠ¢Î“ âˆ™ âŠ¢A) âŠ¢Î” ([tailÏƒ] , [headÏƒ]) =
  let [Î“] , [A] = fundamental âŠ¢A
      [Î”] , [A]â€² , [t] = fundamentalTerm [headÏƒ]
      [Î“]â€² , [Ïƒ] = fundamentalSubst âŠ¢Î“ âŠ¢Î” [tailÏƒ]
      [tailÏƒ]â€² = S.irrelevanceSubst [Î“]â€² [Î“] âŠ¢Î” âŠ¢Î” [Ïƒ]
      [idA]  = projâ‚ (unwrap [A]â€² (soundContext [Î”]) (idSubstS [Î”]))
      [idA]â€² = projâ‚ (unwrap [A] âŠ¢Î” [tailÏƒ]â€²)
      [idt]  = projâ‚ ([t] (soundContext [Î”]) (idSubstS [Î”]))
  in  [Î“] âˆ™ [A] , ([tailÏƒ]â€²
  ,   irrelevanceTermâ€³ (subst-id _) (subst-id _) [idA] [idA]â€² [idt])

-- Fundamental theorem for substitution equality.
fundamentalSubstEq : (âŠ¢Î“ : âŠ¢ Î“) (âŠ¢Î” : âŠ¢ Î”)
      â†’ Î” âŠ¢Ë¢ Ïƒ â‰¡ Ïƒâ€² âˆ· Î“
      â†’ âˆƒâ‚‚ Î» [Î“] [Ïƒ]
      â†’ âˆƒ  Î» ([Ïƒâ€²] : Î” âŠ©Ë¢ Ïƒâ€² âˆ· Î“ / [Î“] / âŠ¢Î”)
      â†’ Î” âŠ©Ë¢ Ïƒ â‰¡ Ïƒâ€² âˆ· Î“ / [Î“] / âŠ¢Î” / [Ïƒ]
fundamentalSubstEq Îµ âŠ¢Î” Ïƒ = Îµ , lift tt , lift tt , lift tt
fundamentalSubstEq (âŠ¢Î“ âˆ™ âŠ¢A) âŠ¢Î” (tailÏƒâ‰¡Ïƒâ€² , headÏƒâ‰¡Ïƒâ€²) =
  let [Î“] , [A] = fundamental âŠ¢A
      [Î“]â€² , [tailÏƒ] , [tailÏƒâ€²] , [tailÏƒâ‰¡Ïƒâ€²] = fundamentalSubstEq âŠ¢Î“ âŠ¢Î” tailÏƒâ‰¡Ïƒâ€²
      [Î”] , modelsTermEq [A]â€² [t] [tâ€²] [tâ‰¡tâ€²] = fundamentalTermEq headÏƒâ‰¡Ïƒâ€²
      [tailÏƒ]â€² = S.irrelevanceSubst [Î“]â€² [Î“] âŠ¢Î” âŠ¢Î” [tailÏƒ]
      [tailÏƒâ€²]â€² = S.irrelevanceSubst [Î“]â€² [Î“] âŠ¢Î” âŠ¢Î” [tailÏƒâ€²]
      [tailÏƒâ‰¡Ïƒâ€²]â€² = S.irrelevanceSubstEq [Î“]â€² [Î“] âŠ¢Î” âŠ¢Î” [tailÏƒ] [tailÏƒ]â€² [tailÏƒâ‰¡Ïƒâ€²]
      [idA]  = projâ‚ (unwrap [A]â€² (soundContext [Î”]) (idSubstS [Î”]))
      [idA]â€² = projâ‚ (unwrap [A] âŠ¢Î” [tailÏƒ]â€²)
      [idA]â€³ = projâ‚ (unwrap [A] âŠ¢Î” [tailÏƒâ€²]â€²)
      [idt]  = projâ‚ ([t] (soundContext [Î”]) (idSubstS [Î”]))
      [idtâ€²] = projâ‚ ([tâ€²] (soundContext [Î”]) (idSubstS [Î”]))
      [idtâ‰¡tâ€²]  = [tâ‰¡tâ€²] (soundContext [Î”]) (idSubstS [Î”])
  in  [Î“] âˆ™ [A]
  ,   ([tailÏƒ]â€² , irrelevanceTermâ€³ (subst-id _) (subst-id _) [idA] [idA]â€² [idt])
  ,   ([tailÏƒâ€²]â€² , convTermâ‚ [idA]â€² [idA]â€³
                             (projâ‚‚ (unwrap [A] âŠ¢Î” [tailÏƒ]â€²) [tailÏƒâ€²]â€² [tailÏƒâ‰¡Ïƒâ€²]â€²)
                             (irrelevanceTermâ€³ (subst-id _) (subst-id _)
                                                [idA] [idA]â€² [idtâ€²]))
  ,   ([tailÏƒâ‰¡Ïƒâ€²]â€² , irrelevanceEqTermâ€³ (subst-id _) (subst-id _) (subst-id _)
                                         [idA] [idA]â€² [idtâ‰¡tâ€²])

opaque
  unfolding _âŠ©áµ›âŸ¨_âŸ©_

  -- A variant of fundamental.

  fundamental-âŠ©áµ› : Î“ âŠ¢ A â†’ Î“ âŠ©áµ›âŸ¨ Â¹ âŸ© A
  fundamental-âŠ©áµ› = fundamental

opaque
  unfolding _âŠ©áµ›âŸ¨_âŸ©_â‰¡_

  -- A variant of fundamentalEq.

  fundamental-âŠ©áµ›â‰¡ : Î“ âŠ¢ A â‰¡ B â†’ Î“ âŠ©áµ›âŸ¨ Â¹ âŸ© A â‰¡ B
  fundamental-âŠ©áµ›â‰¡ = fundamentalEq

opaque
  unfolding _âŠ©áµ›âŸ¨_âŸ©_âˆ·_

  -- A variant of fundamentalTerm.

  fundamental-âŠ©áµ›âˆ· : Î“ âŠ¢ t âˆ· A â†’ Î“ âŠ©áµ›âŸ¨ Â¹ âŸ© t âˆ· A
  fundamental-âŠ©áµ›âˆ· = fundamentalTerm

opaque
  unfolding _âŠ©áµ›âŸ¨_âŸ©_â‰¡_âˆ·_

  -- A variant of fundamentalTermEq.

  fundamental-âŠ©áµ›â‰¡âˆ· : Î“ âŠ¢ t â‰¡ u âˆ· A â†’ Î“ âŠ©áµ›âŸ¨ Â¹ âŸ© t â‰¡ u âˆ· A
  fundamental-âŠ©áµ›â‰¡âˆ· = fundamentalTermEq

opaque
  unfolding _âŠ©Ë¢_âˆ·_

  -- A variant of fundamentalSubst.

  fundamental-âŠ©Ë¢âˆ· : âŠ¢ Î” â†’ âŠ¢ Î“ â†’ Î” âŠ¢Ë¢ Ïƒ âˆ· Î“ â†’ Î” âŠ©Ë¢ Ïƒ âˆ· Î“
  fundamental-âŠ©Ë¢âˆ· âŠ¢Î” âŠ¢Î“ âŠ¢Ïƒ =
    case fundamentalSubst âŠ¢Î“ âŠ¢Î” âŠ¢Ïƒ of Î»
      (_ , âŠ©Ïƒ) â†’
    _ , _ , âŠ©Ïƒ

opaque
  unfolding _âŠ©Ë¢_â‰¡_âˆ·_

  -- A variant of fundamentalSubstEq.

  fundamental-âŠ©Ë¢â‰¡âˆ· : âŠ¢ Î” â†’ âŠ¢ Î“ â†’ Î” âŠ¢Ë¢ Ïƒâ‚ â‰¡ Ïƒâ‚‚ âˆ· Î“ â†’ Î” âŠ©Ë¢ Ïƒâ‚ â‰¡ Ïƒâ‚‚ âˆ· Î“
  fundamental-âŠ©Ë¢â‰¡âˆ· âŠ¢Î” âŠ¢Î“ Ïƒâ‚â‰¡Ïƒâ‚‚ =
    case fundamentalSubstEq âŠ¢Î“ âŠ¢Î” Ïƒâ‚â‰¡Ïƒâ‚‚ of Î»
      (_ , Ïƒâ‚â‰¡Ïƒâ‚‚) â†’
    _ , _ , Ïƒâ‚â‰¡Ïƒâ‚‚
