------------------------------------------------------------------------
-- Admissible rules related to Î£-types
------------------------------------------------------------------------

open import Definition.Typed.Restrictions
open import Graded.Modality

module Definition.Typed.Consequences.Admissible.Sigma
  {a} {M : Set a}
  {ğ•„ : Modality M}
  (R : Type-restrictions ğ•„)
  where

open Type-restrictions R

open import Definition.Typed R
open import Definition.Typed.Consequences.Inequality R
open import Definition.Typed.Consequences.Injectivity R
open import Definition.Typed.Consequences.Inversion R
open import Definition.Typed.EqRelInstance R
open import Definition.Typed.Inversion R
open import Definition.Typed.Properties R
open import Definition.Typed.Substitution R
open import Definition.Typed.Syntactic R

open import Definition.Untyped M
open import Definition.Untyped.Neutral M type-variant
open import Definition.Untyped.Sigma ğ•„

open import Tools.Fin
open import Tools.Function
open import Tools.Product
open import Tools.Relation

private variable
  âˆ‡             : DCon _ _
  Î“             : Con _ _
  A B C t u v w : Term _
  p q qâ€² r      : M
  s             : Strength

------------------------------------------------------------------------
-- Some admissible rules

opaque

  -- A variant of the reduction rule prodrec-Î².

  prodrec-Î²-â‡’â‚ :
    â¦ƒ ok : No-equality-reflection or-empty Î“ â¦„ â†’
    âˆ‡ Â» Î“ âˆ™ (Î£Ê· p , qâ€² â–· A â–¹ B) âŠ¢ C â†’
    âˆ‡ Â» Î“ âŠ¢ prodÊ· p t u âˆ· Î£Ê· p , qâ€² â–· A â–¹ B â†’
    âˆ‡ Â» Î“ âˆ™ A âˆ™ B âŠ¢ v âˆ· C [ prodÊ· p (var x1) (var x0) ]â†‘Â² â†’
    âˆ‡ Â» Î“ âŠ¢ prodrec r p q C (prodÊ· p t u) v â‡’ v [ t , u ]â‚â‚€ âˆ·
      C [ prodÊ· p t u ]â‚€
  prodrec-Î²-â‡’â‚ âŠ¢C âŠ¢p âŠ¢v =
    case inversion-prod âŠ¢p of Î»
      (F , G , q , _ , _ , âŠ¢t , âŠ¢u , Î£â‰¡Î£â€² , _) â†’
    case Î Î£-injectivity Î£â‰¡Î£â€² of Î»
      (Aâ‰¡F , Bâ‰¡G , _) â†’
    case conv âŠ¢t (sym Aâ‰¡F) of Î»
      âŠ¢tâ€² â†’
    prodrec-Î²-â‡’ âŠ¢C âŠ¢tâ€² (conv âŠ¢u (sym (Bâ‰¡G (refl âŠ¢tâ€²)))) âŠ¢v

opaque

  -- A variant of the equality rule prodrec-Î².

  prodrec-Î²-â‰¡â‚ :
    â¦ƒ ok : No-equality-reflection or-empty Î“ â¦„ â†’
    âˆ‡ Â» Î“ âˆ™ (Î£Ê· p , qâ€² â–· A â–¹ B) âŠ¢ C â†’
    âˆ‡ Â» Î“ âŠ¢ prodÊ· p t u âˆ· Î£Ê· p , qâ€² â–· A â–¹ B â†’
    âˆ‡ Â» Î“ âˆ™ A âˆ™ B âŠ¢ v âˆ· C [ prodÊ· p (var x1) (var x0) ]â†‘Â² â†’
    âˆ‡ Â» Î“ âŠ¢ prodrec r p q C (prodÊ· p t u) v â‰¡ v [ t , u ]â‚â‚€ âˆ·
      C [ prodÊ· p t u ]â‚€
  prodrec-Î²-â‰¡â‚ âŠ¢C âŠ¢p âŠ¢v =
    subsetTerm (prodrec-Î²-â‡’â‚ âŠ¢C âŠ¢p âŠ¢v)

-- An "inverse" of prod-cong for Î£Ë¢.

prod-congâ»Â¹-Î£Ë¢ :
  â¦ƒ ok : No-equality-reflection or-empty Î“ â¦„ â†’
  âˆ‡ Â» Î“ âŠ¢ prodË¢ p t u â‰¡ prodË¢ p v w âˆ· Î£Ë¢ p , q â–· A â–¹ B â†’
  (âˆ‡ Â» Î“ âˆ™ A âŠ¢ B) Ã— âˆ‡ Â» Î“ âŠ¢ t â‰¡ v âˆ· A Ã— âˆ‡ Â» Î“ âŠ¢ u â‰¡ w âˆ· B [ t ]â‚€ Ã—
  Î£Ë¢-allowed p q
prod-congâ»Â¹-Î£Ë¢
  {Î“ = Î“} {âˆ‡ = âˆ‡} {p = p} {t = t} {u = u} {v = v} {w = w}
  {q = q} {A = A} {B = B} prodâ‰¡prod =
  âŠ¢B , tâ‰¡v , uâ‰¡w , ok
  where
  âŠ¢Î£AB = syntacticEqTerm prodâ‰¡prod .projâ‚
  âŠ¢B   = inversion-Î Î£ âŠ¢Î£AB .projâ‚‚ .projâ‚
  ok   = inversion-Î Î£ âŠ¢Î£AB .projâ‚‚ .projâ‚‚
  âŠ¢t,u = syntacticEqTerm prodâ‰¡prod .projâ‚‚ .projâ‚
  âŠ¢t   = inversion-prod-Î£ âŠ¢t,u .projâ‚
  âŠ¢u   = inversion-prod-Î£ âŠ¢t,u .projâ‚‚ .projâ‚
  âŠ¢v,w = syntacticEqTerm prodâ‰¡prod .projâ‚‚ .projâ‚‚
  âŠ¢v   = inversion-prod-Î£ âŠ¢v,w .projâ‚
  âŠ¢w   = inversion-prod-Î£ âŠ¢v,w .projâ‚‚ .projâ‚

  fst-t,uâ‰¡t = Î£-Î²â‚-â‰¡ âŠ¢B âŠ¢t âŠ¢u ok

  tâ‰¡v =                                                    $âŸ¨ prodâ‰¡prod âŸ©
    âˆ‡ Â» Î“ âŠ¢ prodË¢ p t u â‰¡ prodË¢ p v w âˆ· Î£Ë¢ p , q â–· A â–¹ B   â†’âŸ¨ fst-congâ€² âŸ©
    âˆ‡ Â» Î“ âŠ¢ fst p (prodË¢ p t u) â‰¡ fst p (prodË¢ p v w) âˆ· A  â†’âŸ¨ (Î» hyp â†’ trans (symâ€² fst-t,uâ‰¡t) (trans hyp (Î£-Î²â‚-â‰¡ âŠ¢B âŠ¢v âŠ¢w ok))) âŸ©
    âˆ‡ Â» Î“ âŠ¢ t â‰¡ v âˆ· A                                      â–¡

  uâ‰¡w =                                                   $âŸ¨ prodâ‰¡prod âŸ©
    âˆ‡ Â» Î“ âŠ¢ prodË¢ p t u â‰¡ prodË¢ p v w âˆ· Î£Ë¢ p , q â–· A â–¹ B  â†’âŸ¨ snd-congâ€² âŸ©

    âˆ‡ Â» Î“ âŠ¢ snd p (prodË¢ p t u) â‰¡ snd p (prodË¢ p v w) âˆ·
      B [ fst p (prodË¢ p t u) ]â‚€                          â†’âŸ¨ (Î» hyp â†’ trans
                                                               (symâ€² (Î£-Î²â‚‚-â‰¡ âŠ¢B âŠ¢t âŠ¢u ok))
                                                                  (trans hyp
                                                                     (conv (Î£-Î²â‚‚-â‰¡ âŠ¢B âŠ¢v âŠ¢w ok)
                                                                        (substTypeEq (refl âŠ¢B)
                                                                           (fst-congâ€² (symâ€² prodâ‰¡prod)))))) âŸ©

    âˆ‡ Â» Î“ âŠ¢ u â‰¡ w âˆ· B [ fst p (prodË¢ p t u) ]â‚€            â†’âŸ¨ flip _âŠ¢_â‰¡_âˆ·_.conv (substTypeEq (refl âŠ¢B) fst-t,uâ‰¡t) âŸ©

    âˆ‡ Â» Î“ âŠ¢ u â‰¡ w âˆ· B [ t ]â‚€                              â–¡

-- An "inverse" of prod-cong for Î£Ê·.

prod-congâ»Â¹-Î£Ê· :
  â¦ƒ ok : No-equality-reflection or-empty Î“ â¦„ â†’
  âˆ‡ Â» Î“ âŠ¢ prodÊ· p t u â‰¡ prodÊ· p v w âˆ· Î£Ê· p , q â–· A â–¹ B â†’
  (âˆ‡ Â» Î“ âˆ™ A âŠ¢ B) Ã— âˆ‡ Â» Î“ âŠ¢ t â‰¡ v âˆ· A Ã— âˆ‡ Â» Î“ âŠ¢ u â‰¡ w âˆ· B [ t ]â‚€ Ã—
  Î£Ê·-allowed p q
prod-congâ»Â¹-Î£Ê·
  {Î“ = Î“} {âˆ‡ = âˆ‡} {p = p} {t = t} {u = u} {v = v} {w = w}
  {q = q} {A = A} {B = B} prodâ‰¡prod =
  âŠ¢B , tâ‰¡v , uâ‰¡w , ok
  where
  âŠ¢Î£AB = syntacticEqTerm prodâ‰¡prod .projâ‚
  âŠ¢A   = inversion-Î Î£ âŠ¢Î£AB .projâ‚
  âŠ¢B   = inversion-Î Î£ âŠ¢Î£AB .projâ‚‚ .projâ‚
  ok   = inversion-Î Î£ âŠ¢Î£AB .projâ‚‚ .projâ‚‚
  âŠ¢t,u = syntacticEqTerm prodâ‰¡prod .projâ‚‚ .projâ‚
  âŠ¢t   = inversion-prod-Î£ âŠ¢t,u .projâ‚
  âŠ¢u   = inversion-prod-Î£ âŠ¢t,u .projâ‚‚ .projâ‚
  âŠ¢v,w = syntacticEqTerm prodâ‰¡prod .projâ‚‚ .projâ‚‚
  âŠ¢v   = inversion-prod-Î£ âŠ¢v,w .projâ‚
  âŠ¢w   = inversion-prod-Î£ âŠ¢v,w .projâ‚‚ .projâ‚

  fst-t,uâ‰¡t = fstÊ·-Î²-â‰¡ âŠ¢B âŠ¢t âŠ¢u ok

  tâ‰¡v =                                                          $âŸ¨ prodâ‰¡prod âŸ©
    âˆ‡ Â» Î“ âŠ¢ prodÊ· p t u â‰¡ prodÊ· p v w âˆ· Î£Ê· p , q â–· A â–¹ B         â†’âŸ¨ fstÊ·-cong (refl âŠ¢A) âŸ©
    âˆ‡ Â» Î“ âŠ¢ fstÊ· p A (prodÊ· p t u) â‰¡ fstÊ· p A (prodÊ· p v w) âˆ· A  â†’âŸ¨ (Î» hyp â†’ trans (symâ€² fst-t,uâ‰¡t)
                                                                   (trans hyp (fstÊ·-Î²-â‰¡ âŠ¢B âŠ¢v âŠ¢w ok))) âŸ©
    âˆ‡ Â» Î“ âŠ¢ t â‰¡ v âˆ· A                                            â–¡

  uâ‰¡w =                                                                $âŸ¨ prodâ‰¡prod âŸ©
    âˆ‡ Â» Î“ âŠ¢ prodÊ· p t u â‰¡ prodÊ· p v w âˆ· Î£Ê· p , q â–· A â–¹ B               â†’âŸ¨ sndÊ·-cong (refl âŠ¢A) (refl âŠ¢B) âŸ©

    âˆ‡ Â» Î“ âŠ¢ sndÊ· p q A B (prodÊ· p t u) â‰¡ sndÊ· p q A B (prodÊ· p v w) âˆ·
      B [ fstÊ· p A (prodÊ· p t u) ]â‚€                                    â†’âŸ¨ (Î» hyp â†’ trans
                                                                             (symâ€² (sndÊ·-Î²-â‰¡ âŠ¢B âŠ¢t âŠ¢u ok))
                                                                                (trans hyp
                                                                                   (conv (sndÊ·-Î²-â‰¡ âŠ¢B âŠ¢v âŠ¢w ok)
                                                                                      (substTypeEq (refl âŠ¢B)
                                                                                         (fstÊ·-cong (refl âŠ¢A) (symâ€² prodâ‰¡prod)))))) âŸ©

    âˆ‡ Â» Î“ âŠ¢ u â‰¡ w âˆ· B [ fstÊ· p A (prodÊ· p t u) ]â‚€                      â†’âŸ¨ flip _âŠ¢_â‰¡_âˆ·_.conv (substTypeEq (refl âŠ¢B) fst-t,uâ‰¡t) âŸ©

    âˆ‡ Â» Î“ âŠ¢ u â‰¡ w âˆ· B [ t ]â‚€                                           â–¡

-- An "inverse" of prod-cong.

prod-congâ»Â¹ :
  â¦ƒ ok : No-equality-reflection or-empty Î“ â¦„ â†’
  âˆ‡ Â» Î“ âŠ¢ prod s p t u â‰¡ prod s p v w âˆ· Î£âŸ¨ s âŸ© p , q â–· A â–¹ B â†’
  (âˆ‡ Â» Î“ âˆ™ A âŠ¢ B) Ã— âˆ‡ Â» Î“ âŠ¢ t â‰¡ v âˆ· A Ã— âˆ‡ Â» Î“ âŠ¢ u â‰¡ w âˆ· B [ t ]â‚€ Ã—
  Î£-allowed s p q
prod-congâ»Â¹ {s = ğ•¤} = prod-congâ»Â¹-Î£Ë¢
prod-congâ»Â¹ {s = ğ•¨} = prod-congâ»Â¹-Î£Ê·

------------------------------------------------------------------------
-- Negative results related to Î·-rules for Î£Ê·

-- If Î£Ê·-allowedÂ pÂ q holds for some p andÂ q, and equality reflection
-- is not allowed, then a certain definitional Î·-rule for Î£Ê·, fstÊ· and
-- sndÊ· does not hold in general.
--
-- See also
-- Definition.Typed.Properties.Admissible.Sigma.âŠ¢Î£Ê·-Î·-prodÊ·-fstÊ·-sndÊ·.

Â¬-Î£Ê·-Î·-prodÊ·-fstÊ·-sndÊ· :
  â¦ƒ not-ok : No-equality-reflection â¦„ â†’
  Î£Ê·-allowed p q â†’
  Â¬ (âˆ€ {m n} {âˆ‡ : DCon (Term 0) m} {Î“ : Con Term n} {t A B} â†’
     âˆ‡ Â» Î“ âŠ¢ t âˆ· Î£Ê· p , q â–· A â–¹ B â†’
     âˆ‡ Â» Î“ âŠ¢ prodÊ· p (fstÊ· p A t) (sndÊ· p q A B t) â‰¡ t âˆ· Î£Ê· p , q â–· A â–¹ B)
Â¬-Î£Ê·-Î·-prodÊ·-fstÊ·-sndÊ· {p = p} {q = q} Î£-ok hyp = Â¬fst,sndâ‰¡ fst,sndâ‰¡
  where
  Aâ€² = â„•
  Bâ€² = â„•

  Î“â€² = Îµ âˆ™ Î£Ê· p , q â–· â„• â–¹ â„•

  tâ€² : Term 1
  tâ€² = var x0

  âŠ¢Î“ : Îµ Â»âŠ¢ Î“â€²
  âŠ¢Î“ = âˆ™ Î Î£â±¼ (â„•â±¼ (âˆ™ â„•â±¼ ÎµÎµ)) Î£-ok

  âŠ¢B : Îµ Â» Î“â€² âˆ™ Aâ€² âŠ¢ Bâ€²
  âŠ¢B = â„•â±¼ (âˆ™ â„•â±¼ âŠ¢Î“)

  âŠ¢t : Îµ Â» Î“â€² âŠ¢ tâ€² âˆ· Î£Ê· p , q â–· Aâ€² â–¹ Bâ€²
  âŠ¢t = var âŠ¢Î“ here

  fst,sndâ‰¡ :
    Îµ Â» Î“â€² âŠ¢ prodÊ· p (fstÊ· p Aâ€² tâ€²) (sndÊ· p q Aâ€² Bâ€² tâ€²) â‰¡ tâ€² âˆ·
      Î£Ê· p , q â–· Aâ€² â–¹ Bâ€²
  fst,sndâ‰¡ = hyp âŠ¢t

  Â¬fst,sndâ‰¡ :
    Â¬ Îµ Â» Î“â€² âŠ¢ prodÊ· p (fstÊ· p Aâ€² tâ€²) (sndÊ· p q Aâ€² Bâ€² tâ€²) â‰¡ tâ€² âˆ·
        Î£Ê· p , q â–· Aâ€² â–¹ Bâ€²
  Â¬fst,sndâ‰¡ = prodÊ·â‰¢ne â¦ƒ ok = included â¦„ _ (varâº _)

-- If Î£Ê·-allowedÂ pÂ q holds for some p andÂ q, and equality reflection
-- is not allowed, then a certain definitional Î·-rule for Î£Ê·, fstÊ· and
-- sndÊ· does not hold in general.

Â¬-Î£Ê·-Î· :
  â¦ƒ not-ok : No-equality-reflection â¦„ â†’
  Î£Ê·-allowed p q â†’
  Â¬ (âˆ€ {m n} {âˆ‡ : DCon (Term 0) m} {Î“ : Con Term n} {t A B u} â†’
     âˆ‡ Â» Î“ âŠ¢ t âˆ· Î£Ê· p , q â–· A â–¹ B â†’
     âˆ‡ Â» Î“ âŠ¢ u âˆ· Î£Ê· p , q â–· A â–¹ B â†’
     âˆ‡ Â» Î“ âŠ¢ fstÊ· p A t â‰¡ fstÊ· p A u âˆ· A â†’
     âˆ‡ Â» Î“ âŠ¢ sndÊ· p q A B t â‰¡ sndÊ· p q A B u âˆ· B [ fstÊ· p A t ]â‚€ â†’
     âˆ‡ Â» Î“ âŠ¢ t â‰¡ u âˆ· Î£Ê· p , q â–· A â–¹ B)
Â¬-Î£Ê·-Î· Î£-ok hyp =
  Â¬-Î£Ê·-Î·-prodÊ·-fstÊ·-sndÊ· Î£-ok Î» âŠ¢t â†’
    case inversion-Î Î£ (syntacticTerm âŠ¢t) of Î» {
      (_ , âŠ¢B , ok) â†’
    hyp (prodâ±¼ âŠ¢B (fstÊ·â±¼ âŠ¢t) (sndÊ·â±¼ âŠ¢t) ok) âŠ¢t
      (fstÊ·-Î²-â‰¡ âŠ¢B (fstÊ·â±¼ âŠ¢t) (sndÊ·â±¼ âŠ¢t) ok)
      (sndÊ·-Î²-â‰¡ âŠ¢B (fstÊ·â±¼ âŠ¢t) (sndÊ·â±¼ âŠ¢t) ok) }
